Make the pattern stronger, and make it easier to use

DListRef.fst
@@ -475,7 +475,8 @@ let dlisthead_remove_tail #t h =
 
 #reset-options
 
-let rec get_ref_index (#t:Type) (s:seq (ref t)) (x:ref t{Seq.contains s x}) : GTot nat
+let rec get_ref_index (#t:Type) (s:seq (ref t)) (x:ref t{Seq.contains s x}) :
+  GTot (i:nat{i < Seq.length s})
     (decreases (Seq.length s)) =
   contains_elim s x;
   let h, t = Seq.head s, Seq.tail s in
@@ -485,12 +486,9 @@ let rec get_ref_index (#t:Type) (s:seq (ref t)) (x:ref t{Seq.contains s x}) : GT
 
 val lemma_get_ref_index : #t:Type -> s:seq (ref t) -> x:ref t{Seq.contains s x} ->
   Lemma (ensures (
-    let i = get_ref_index s x in
-    i < Seq.length s /\
-    (let (i:nat{i < Seq.length s}) = i in // more workarounds for two phase
-         addr_of s.[i] = addr_of x)))
+    addr_of s.[get_ref_index s x] = addr_of x))
     (decreases (Seq.length s))
-    [SMTPat (get_ref_index s x)]
+    [SMTPat (addr_of s.[get_ref_index s x])]
 let rec lemma_get_ref_index #t s x =
   contains_elim s x;
   let h, t = Seq.head s, Seq.tail s in
